proof/format_proof.v
@@ -52,6 +52,7 @@ Fixpoint listrep (sigma: list (Z * (list byte))) (p: val) : mpred :=
  match sigma with
  | (a, b)::hs =>
     EX x:val, EX y: val,
+    (emp || malloc_token Ews (Tarray tschar (Zlength b + 1) noattr) y) *
     cstring Ews b y *
     malloc_token Ews t_list p * 
     data_at Ews t_list ((Vint (Int.repr a), (y, x)) : @reptype CompSpecs t_list) p *
@@ -64,6 +65,7 @@ Fixpoint lseg (sigma: list (Z * (list byte))) (x z: val) : mpred :=
   match sigma with
   | nil => !! (x = z) && emp
   | (a, b)::hs => EX h: val, EX y:val, 
+        (emp || malloc_token Ews (Tarray tschar (Zlength b + 1) noattr) y) *
         cstring Ews b y *
         malloc_token Ews t_list x * 
         data_at Ews t_list ((Vint (Int.repr a)), (y, h)) x * 
@@ -74,17 +76,17 @@ Arguments lseg sigma x z : simpl never.
 
 Definition list_copy_spec : ident * funspec :=
 DECLARE _list_copy
-  WITH sh : share, p : val, s : list (Z * (list byte)), gv: globals
+  WITH sh : share, l : val, sigma : list (Z * (list byte)), gv: globals
   PRE [ tptr t_list ]
-    PROP(0 <= Zlength s <= Ptrofs.max_unsigned;
-         Forall (fun x => 0 <= (fst x) <= Int.max_unsigned /\ 0 <= Zlength (snd x) + 1 <= Ptrofs.max_unsigned) s)
-    PARAMS(p) GLOBALS(gv)
-    SEP(listrep s p; mem_mgr gv)
+    PROP(0 <= Zlength sigma <= Int.max_unsigned;
+         Forall (fun x => 0 <= (fst x) <= Int.max_unsigned /\ 0 <= Zlength (snd x) + 1 <= Int.max_unsigned) sigma)
+    PARAMS(l) GLOBALS(gv)
+    SEP(listrep sigma l; mem_mgr gv)
   POST [ tptr t_list ] 
     EX q: val,
-    PROP(p <> nullval -> p <> q)
+    PROP()
     RETURN(q)
-    SEP(listrep s q; listrep s p; mem_mgr gv).
+    SEP(listrep sigma l; listrep sigma q; mem_mgr gv).
 
 
 Definition t_format := Tstruct _t noattr.
@@ -234,10 +236,6 @@ forward_loop  (EX i : Z,
   SEP (data_at sh (tarray tschar (Zlength s + 1))
           (map Vbyte (s ++ [Byte.zero])) str)).
 
-assert (Example: Archi.ptr64=false -> 
-          forall n, Vptrofs (Ptrofs.repr n) = Vint (Int.repr n)).
-{ intro Hx; try discriminate Hx. }
-clear Example.
 { Exists 0. entailer. }
 Intros i. forward. forward_if. forward. entailer!. 
 repeat f_equal. cstring.
@@ -314,7 +312,7 @@ unfold listrep. destruct sigma; simpl.
 destruct p0. Intros x y. auto with valid_pointer.
 Qed.
 #[export] Hint Resolve listrep_valid_pointer : valid_pointer.
-
+  
 Lemma less_components_fact1: 
   forall (x y : nat), 
     (0 <= (Z.of_nat x) <= Int.max_unsigned) ->
@@ -771,6 +769,8 @@ Proof.
     unfold line. simpl.
     repeat rewrite list_byte_to_string_length.
     entailer!.
+    apply orp_right1.
+    entailer.
 Qed.
 
 
@@ -785,35 +785,385 @@ Proof.
     rewrite <- IHt. list_solve.
 Qed.
 
-Lemma list_copy_fact1:
-  forall (A : Type) (i : Z) (t : list A),
-    0 <= i ->
-    skipn (Z.to_nat i) t = sublist i (Zlength t) t.
-Proof.
-  intros. 
-  unfold sublist.
-  f_equal.
-  rewrite list_copy_length_fact.
-  symmetry.
-  apply firstn_exact_length.
-Qed.
-
-Lemma list_copy_fact2:
-  forall (A : Type) (t : list A),
-  Z.to_nat (Zlength t) =  Datatypes.length (firstn (Z.to_nat (Zlength t + 1)) t).
+Lemma singleton_listrep: forall (a : Z) (b : list byte) (h : val) (x: val),
+  cstring Ews b h *
+  malloc_token Ews t_list x *
+  data_at Ews t_list ((Vint (Int.repr a)), (h, nullval)) x
+   |-- listrep [(a, b)] x.
 Proof.
   intros.
-  induction t.
-  - list_solve.
-  - replace (Zlength (a :: t)) with (Zlength t + 1) by list_solve.
-    replace (Z.to_nat (Zlength t + 1 + 1)) with (S (Z.to_nat (Zlength t + 1))) by list_solve.
-    rewrite firstn_cons.
-    simpl.
-    rewrite <- IHt.
-    list_solve.
+  unfold listrep.
+  Exists nullval h.
+  entailer!.
+  apply orp_right1.
+  entailer.
+Qed.
+
+Lemma singleton_lseg: forall (a : Z) (b : list byte) (h : val) (x y: val),
+  cstring Ews b h *
+  malloc_token Ews t_list x *
+  data_at Ews t_list ((Vint (Int.repr a)), (h, y)) x
+   |-- lseg [(a, b)] x y.
+Proof.
+  intros.
+  unfold lseg. 
+  Exists y h.
+  entailer!.
+  apply orp_right1.
+  entailer.
+Qed.
+
+Lemma lseg_list: forall (s1 s2: list (Z * list byte)) (x y: val),
+  lseg s1 x y * listrep s2 y |-- listrep (s1 ++ s2) x.
+Proof.
+  induction s1.
+  - intros. simpl. unfold lseg. entailer!.
+  - intros. simpl. unfold lseg; fold lseg. destruct a.
+    Intros h y0.
+    unfold listrep; fold listrep. Exists h y0.
+    entailer!. apply IHs1.
+Qed.
+
+Lemma lseg_lseg: forall (s1 s2: list (Z * list byte)) (x y z: val),
+  lseg s1 x y * lseg s2 y z |-- lseg (s1 ++ s2) x z.
+Proof.
+  intros s1. induction s1.
+  - intros. unfold lseg; fold lseg. simpl. entailer!.
+  - intros. unfold lseg; fold lseg. destruct a. Intros h y0. simpl.
+    unfold lseg; fold lseg.
+    Exists h y0.
+    assert (
+      (emp || malloc_token Ews (Tarray tschar (Zlength l + 1) noattr) y0)
+        * cstring Ews l y0
+        * malloc_token Ews t_list x
+        * data_at Ews t_list (Vint (Int.repr z0), (y0, h)) x
+        * lseg s1 h y
+        * lseg s2 y z
+        |-- 
+      (emp || malloc_token Ews (Tarray tschar (Zlength l + 1) noattr) y0)
+        * cstring Ews l y0
+        * malloc_token Ews t_list x
+        * data_at Ews t_list (Vint (Int.repr z0), (y0, h)) x
+        * (lseg s1 h y
+        * lseg s2 y z)
+    ) as H by entailer!.
+    eapply (derives_trans _ _ _); eauto.
+    apply sepcon_derives; entailer.
 Qed.
 
 Lemma body_list_copy: semax_body Vprog Gprog f_list_copy list_copy_spec.
 Proof.
-Admitted.
-      
+  start_function.
+  forward_if(l <> nullval). {
+    forward. Exists nullval. entailer!.
+    destruct H2. assert (nullval = nullval) as Trivial by auto.
+    apply H1 in Trivial as sigma_fact.
+    rewrite sigma_fact.
+    unfold listrep.
+    entailer!.
+  }
+  { forward. entailer!. }
+
+  forward_call(t_list, gv).
+  Intros new_pointer.
+  destruct (eq_dec new_pointer nullval). {
+    forward_if(new_pointer <> nullval).
+    { forward_call. entailer!. }
+    { forward. entailer!. } 
+    { forward. contradiction. }
+  }
+
+  forward_if(new_pointer <> nullval).
+  { forward_call. entailer!. }
+  { forward. entailer!. }
+
+  Intros. do 2 forward.
+  
+  forward_loop (
+    EX i : Z, EX cur : val, EX l_cur : val,
+    PROP(0 <= i < Zlength sigma + 1;
+         cur <> nullval;
+         l_cur <> nullval)
+    LOCAL(temp _new new_pointer; 
+          temp _l l;
+          temp _cur cur; 
+          temp _l_cur l_cur; 
+          gvars gv)
+    SEP(malloc_token Ews t_list cur;
+        data_at_ Ews t_list cur;
+        lseg (sublist 0 i sigma) new_pointer cur; 
+        lseg (sublist 0 i sigma) l l_cur;
+        listrep (sublist i (Zlength sigma) sigma) l_cur;
+        mem_mgr gv)
+  ) break: (
+    PROP()
+    LOCAL(temp _new new_pointer; gvars gv)
+    SEP(listrep sigma new_pointer; listrep sigma l; mem_mgr gv)
+  ).
+  3: { forward. Exists new_pointer. entailer!. }
+  {
+    Exists 0 new_pointer l.
+    entailer!.
+    replace (sublist 0 0 sigma) with ([] : list (Z * list byte)) by list_solve.
+    unfold lseg.
+    replace (sublist 0 (Zlength sigma) sigma) with sigma by list_solve.
+    entailer!.
+  }
+  
+  Intros i cur l_cur.
+  rename H2 into I_Boundaries.
+  rename H1 into L_not_null.
+  rename n into New_pointer_not_null.
+  rename H3 into Cur_not_null.
+  rename H4 into L_cur_not_null.
+  destruct (eq_dec i (Zlength sigma)) as [ | I_is_not_zlength]. {
+    subst.
+    replace ((sublist (Zlength sigma) (Zlength sigma) sigma)) with ([] : list (Z * list byte)) by list_solve.
+    unfold listrep; fold listrep. 
+    Intros. contradiction.
+  }
+
+replace (sublist i (Zlength sigma) sigma) with 
+  (Znth i sigma :: sublist (i + 1) (Zlength sigma) sigma) by list_solve.
+unfold listrep; fold listrep.
+remember (Znth i sigma) as ith_element.
+destruct ith_element as (shift_i, line_i).
+
+Intros l_cur_tail line_i_pointer.
+do 3 forward.
+forward_call(Ews, line_i, line_i_pointer).
+forward_call((Tarray tschar (Zlength line_i + 1) noattr), gv). {
+  assert (In (shift_i, line_i) sigma) as In_fact. 
+  { rewrite Heqith_element. apply Znth_In. lia. }
+
+  assert (Zlength line_i + 1 <= Int.max_unsigned) as Zlength_fact. {
+    remember (fun x : Z * list byte =>
+    0 <= fst x <= Int.max_unsigned /\
+    0 <= Zlength (snd x) + 1 <= Int.max_unsigned) as List_condition.
+    assert (List_condition (shift_i, line_i)) as Ith_condition. 
+    { apply (computable_theorems.Forall_forall1 _ sigma); auto. }
+    rewrite HeqList_condition in Ith_condition.
+    destruct Ith_condition as [shift_condition].
+    simpl in H1. lia.
+  }
+
+  unfold sizeof. unfold Ctypes.sizeof.
+  unfold Int.max_unsigned in Zlength_fact. simpl in Zlength_fact.
+  unfold Ptrofs.max_unsigned. simpl.
+  lia.
+}
+
+Intros cur_line_i_pointer.
+destruct (eq_dec cur_line_i_pointer nullval). {
+  do 2 forward.
+  forward_if(cur_line_i_pointer <> nullval).
+  { forward_call. entailer!. }
+  { forward. entailer!. }
+  { forward. contradiction. }
+}
+
+Intros. do 2 forward.
+forward_if(cur_line_i_pointer <> nullval).
+{ forward_call. entailer!. }
+{ forward. entailer!. }
+
+do 2 forward.
+forward_call(Ews, Ews, cur_line_i_pointer, Zlength line_i + 1, line_i_pointer, line_i).
+do 2 forward.
+
+forward_if(l_cur_tail <> nullval). {
+  do 2 forward.
+  entailer!.
+  rewrite <- cstringn_equiv.
+  assert (i + 1 = Zlength sigma) as AA. {
+    assert (i + 1 < Zlength sigma \/ i + 1 = Zlength sigma) as BB. lia.
+    destruct BB. {
+      replace (sublist (i + 1) (Zlength sigma) sigma) 
+        with (Znth (i + 1) sigma :: (sublist (i + 2) (Zlength sigma) sigma)) in H12 by list_solve.
+        destruct H12.
+      assert( Znth (i + 1) sigma :: sublist (i + 2) (Zlength sigma) sigma = []) as CC by auto.
+      inversion CC.
+    }
+    auto.
+  }
+  rewrite AA.
+  replace (sublist (Zlength sigma) (Zlength sigma) sigma) with ([] : list (Z * list byte)) by list_solve.
+  unfold listrep; fold listrep.
+  
+  entailer!.
+
+  assert (
+    cstring Ews line_i cur_line_i_pointer 
+      * cstring Ews line_i line_i_pointer
+      * malloc_token Ews (Tarray tschar (Zlength line_i + 1) noattr) cur_line_i_pointer
+      * malloc_token Ews t_list cur
+      * data_at Ews t_list (Vint (Int.repr shift_i), (cur_line_i_pointer, Vlong (Int64.repr 0))) cur
+      * lseg (sublist 0 i sigma) new_pointer cur
+      * lseg (sublist 0 i sigma) l l_cur
+      * (emp || malloc_token Ews (Tarray tschar (Zlength line_i + 1) noattr) line_i_pointer)
+      * malloc_token Ews t_list l_cur
+      * data_at Ews t_list (Vint (Int.repr shift_i), (line_i_pointer, nullval)) l_cur
+    |-- 
+    (lseg (sublist 0 i sigma) new_pointer cur *
+    (
+      malloc_token Ews (Tarray tschar (Zlength line_i + 1) noattr) cur_line_i_pointer
+      * cstring Ews line_i cur_line_i_pointer 
+      * malloc_token Ews t_list cur
+      * data_at Ews t_list (Vint (Int.repr shift_i), (cur_line_i_pointer, Vlong (Int64.repr 0))) cur
+    )) * (
+      lseg (sublist 0 i sigma) l l_cur *
+      (
+      (emp || malloc_token Ews (Tarray tschar (Zlength line_i + 1) noattr) line_i_pointer)
+      * cstring Ews line_i line_i_pointer
+      * malloc_token Ews t_list l_cur
+      * data_at Ews t_list (Vint (Int.repr shift_i), (line_i_pointer, nullval)) l_cur
+      )
+    )
+  ) as Trans_step1. 
+  { entailer!. }
+
+  eapply (derives_trans _ _ _); eauto. 
+  apply sepcon_derives. 
+  {
+    assert (sigma = sublist 0 i sigma ++ sublist i (Zlength sigma) sigma) as FF by list_solve.
+    rewrite FF.
+    assert (
+      lseg (sublist 0 i (sublist 0 i sigma ++ sublist i (Zlength sigma) sigma)) new_pointer cur
+       * (malloc_token Ews (Tarray tschar (Zlength line_i + 1) noattr) cur_line_i_pointer
+       * cstring Ews line_i cur_line_i_pointer
+       * malloc_token Ews t_list cur
+       * data_at Ews t_list (Vint (Int.repr shift_i), (cur_line_i_pointer, Vlong (Int64.repr 0))) cur)
+       |-- 
+      lseg (sublist 0 i (sublist 0 i sigma ++ sublist i (Zlength sigma) sigma)) new_pointer cur *
+      listrep [(shift_i, line_i)] cur
+    ) as Trans_step2. {
+      unfold listrep; fold listrep.
+      Exists nullval cur_line_i_pointer.
+      entailer!. apply orp_right2. entailer.
+    }
+
+    eapply (derives_trans _ _ _); eauto.
+    rewrite Heqith_element.
+    replace [Znth i sigma] with (sublist i (Zlength sigma) sigma) by list_solve.
+    replace (sublist 0 i sigma ++ sublist i (Zlength sigma) sigma) with sigma at 1 by list_solve.
+    apply lseg_list.
+  }
+  {
+    assert (sigma = sublist 0 i sigma ++ sublist i (Zlength sigma) sigma) as FF by list_solve.
+    rewrite FF.
+    assert (
+      lseg (sublist 0 i (sublist 0 i sigma ++ sublist i (Zlength sigma) sigma)) l l_cur
+        * ((emp || malloc_token Ews (Tarray tschar (Zlength line_i + 1) noattr) line_i_pointer)
+          * cstring Ews line_i line_i_pointer
+          * malloc_token Ews t_list l_cur
+          * data_at Ews t_list (Vint (Int.repr shift_i), (line_i_pointer, nullval)) l_cur)
+      |-- 
+      lseg (sublist 0 i (sublist 0 i sigma ++ sublist i (Zlength sigma) sigma)) l l_cur *
+      listrep [(shift_i, line_i)] l_cur
+    ) as Trans_step2. {
+      unfold listrep; fold listrep.
+      Exists nullval line_i_pointer.
+      entailer!.
+    }
+
+    eapply (derives_trans _ _ _); eauto.
+    rewrite Heqith_element.
+    replace [Znth i sigma] with (sublist i (Zlength sigma) sigma) by list_solve.
+    replace (sublist 0 i sigma ++ sublist i (Zlength sigma) sigma) with sigma at 1 by list_solve.
+    apply lseg_list.
+  }
+  }
+  { forward. entailer!. }
+  Intros.
+  forward_call(t_list, gv).
+  Intros cur_tail.
+  do 2 forward.
+  destruct (eq_dec cur_tail nullval). {
+    forward_if(cur_tail <> nullval).
+    { forward_call. entailer!. }
+    { forward. entailer!. }
+    { forward. contradiction. }
+  }
+  forward_if(cur_tail <> nullval). 
+  { forward_call. entailer!. }
+  { forward. entailer!. }
+  Intros.
+
+  do 2 forward.
+  Exists (i + 1) cur_tail l_cur_tail.
+  entailer!.
+  rewrite <- cstringn_equiv.
+
+  assert (
+    cstring Ews line_i cur_line_i_pointer * cstring Ews line_i line_i_pointer
+    * malloc_token Ews (Tarray tschar (Zlength line_i + 1) noattr) cur_line_i_pointer
+    * malloc_token Ews t_list cur
+    * data_at Ews t_list (Vint (Int.repr shift_i), (cur_line_i_pointer, cur_tail)) cur
+    * lseg (sublist 0 i sigma) new_pointer cur
+    * lseg (sublist 0 i sigma) l l_cur
+    * (emp || malloc_token Ews (Tarray tschar (Zlength line_i + 1) noattr) line_i_pointer)
+    * malloc_token Ews t_list l_cur
+    * data_at Ews t_list (Vint (Int.repr shift_i), (line_i_pointer, l_cur_tail)) l_cur
+    |--
+    (lseg (sublist 0 i sigma) new_pointer cur
+    * (malloc_token Ews (Tarray tschar (Zlength line_i + 1) noattr) cur_line_i_pointer
+    * cstring Ews line_i cur_line_i_pointer
+    * malloc_token Ews t_list cur
+    * data_at Ews t_list (Vint (Int.repr shift_i), (cur_line_i_pointer, cur_tail)) cur))
+    * (lseg (sublist 0 i sigma) l l_cur
+    * ((emp || malloc_token Ews (Tarray tschar (Zlength line_i + 1) noattr) line_i_pointer)
+    * cstring Ews line_i line_i_pointer
+    * malloc_token Ews t_list l_cur
+    * data_at Ews t_list (Vint (Int.repr shift_i), (line_i_pointer, l_cur_tail)) l_cur))
+  ) as AA by entailer!.
+  
+  eapply (derives_trans _ _ _); eauto.
+  apply sepcon_derives. {
+    clear AA.
+    assert (
+      lseg (sublist 0 i sigma) new_pointer cur
+       * (malloc_token Ews (Tarray tschar (Zlength line_i + 1) noattr) cur_line_i_pointer
+       * cstring Ews line_i cur_line_i_pointer
+       * malloc_token Ews t_list cur
+       * data_at Ews t_list (Vint (Int.repr shift_i), (cur_line_i_pointer, cur_tail)) cur)
+      |-- 
+      lseg (sublist 0 i sigma) new_pointer cur * 
+      lseg (sublist i (i + 1) sigma) cur cur_tail
+    ). {
+      apply sepcon_derives. entailer.
+      replace (sublist i (i + 1) sigma) with [Znth i sigma] by list_solve.
+      unfold lseg.
+      rewrite <- Heqith_element.
+      Exists cur_tail cur_line_i_pointer.
+      entailer!.
+      apply orp_right2. entailer.
+    }
+    eapply (derives_trans _ _ _); eauto.
+    replace (sublist 0 (i + 1) sigma) with (sublist 0 i sigma ++ sublist i (i + 1) sigma) by list_solve.
+    apply lseg_lseg.
+  }
+  {
+    clear AA.
+    assert (
+      lseg (sublist 0 i sigma) l l_cur
+      * ((emp || malloc_token Ews (Tarray tschar (Zlength line_i + 1) noattr) line_i_pointer)
+      * cstring Ews line_i line_i_pointer
+      * malloc_token Ews t_list l_cur
+      * data_at Ews t_list (Vint (Int.repr shift_i), (line_i_pointer, l_cur_tail)) l_cur)
+      |-- 
+      lseg (sublist 0 i sigma) l l_cur * 
+      lseg (sublist i (i + 1) sigma) l_cur l_cur_tail
+    ). {
+      apply sepcon_derives. entailer.
+      replace (sublist i (i + 1) sigma) with [Znth i sigma] by list_solve.
+      unfold lseg.
+      rewrite <- Heqith_element.
+      Exists l_cur_tail line_i_pointer.
+      entailer!.
+    }
+    eapply (derives_trans _ _ _); eauto.
+    replace (sublist 0 (i + 1) sigma) with (sublist 0 i sigma ++ sublist i (i + 1) sigma) by list_solve.
+    apply lseg_lseg.
+  }
+Qed.
+
